%        File: assg1.tex
%     Created: Wed Oct 06 08:00 PM 2010 P
% Last Change: Wed Oct 06 08:00 PM 2010 P
%
\documentclass[a4paper,12pt]{article}
\usepackage{amsmath}
\begin{document}
\noindent Matt Forbes \\
October 7 \\
Homework 1 \\


\section{Problem One}
\subsection{}
The minimum number of socks that need to be drawn to guarantee a pair of any color is 4.
You could possibly have 3 socks that do not make a pair, but on the next draw, one of the 
socks will become a match.
\subsection{}
Likewise, the minimum number of socks from a drawer of n different color socks (assuming there is at least 2 of each color)
is n+1. For the same reason that you can have no match on the nth draw, but on the n+1th draw, one sock will match.

\section{Problem Two}
Prove by induction that \(F_{n+k} = F_kF_{n+1} + F_{k-1}F_n\)
\subsection{Basis}
\begin{align*}
  \text{let n=0, k \(>=\) 1} \\
  F_{0+k} = F_kF_1 + F_{k-1}F_0 \\
  F_k = F_k(1) + F_{k-1}(0) \\
  F_k = F_k
\end{align*}

\subsection{Inductive Hypothesis}
For all \(n >= 1, c >= 0 \), assuming the equation is true for \(n-1\) then it 
is also true for \(n\).

\subsection{Proof}
\begin{eqnarray*}
  F_{n+c} &=& F_cF_{n+1} + F_{c-1}F_n \\
  F_{(n-1) + (c+1)} &=& F_cF_{n+1} + F_{c-1}F_n \\
  F_{c+1}F_n + F_cF_{n-1} &=& F_c(F_{n-1} + F_n) + F_{c-1}F_n \\
  (F_{c-1} + F_c)F_n + F_cF_{n-1} &=& F_cF_{n-1} + F_cF_n + F_{c-1}F_n \\
  F_{c-1}F_n + F_cF_n + F_cF_{n-1} &=& F_{c-1}F_n + F_cF_n + F_cF_{n-1} \\
\end{eqnarray*}

\section{Problem Three}
Prove \(\sum_{i=0}^{n} \dbinom{n}{i} = 2^n\) with induction and given identity.
\subsection{Basis}
\begin{eqnarray*}
  \sum_{i=0}^{1} \dbinom{1}{i} &=& \dbinom{1}{0} + \dbinom{1}{1} \\
  &=& 1 + 1 \\
  &=& 2^1 \\
\end{eqnarray*}
\subsection{Inductive Hypothesis}
For all \(n > 1\), assuming the sum is true for \(n-1\), it is also true for \(n\).
\subsection{Induction}
\begin{eqnarray*}
  \sum_{i=0}^{n} \dbinom{n}{i} &=& \dbinom{n}{0} + \sum_{i=1}^{n} \dbinom{n}{i} \text{[pull first value from sum]} \\
  &=& 1 + \sum_{i=1}^{n} \dbinom{n-1}{i} + \dbinom{n-1}{i-1} \text{[given identity]} \\
  &=& 1 + \sum_{i=1}^{n} \dbinom{n-1}{i} + \sum_{i=1}^{n} \dbinom{n-1}{i-1} \text{[break up sum]} \\
  &=& 1 + [(\sum_{i=0}^{n} \dbinom{n-1}{i}) - \dbinom{n}{0}] + \sum_{i=0}^{n} \dbinom{n-1}{i} \text{[change sum limits]} \\
  &=& 1 + [2^{n-1} - 1] + 2^{n-1} \text{[inductive hypthosis]} \\
  &=& 2*2^{n-1} \\
  &=& 2^n
\end{eqnarray*}
\section{Problem Four}

\end{document}


